LeanMqtt/Primitives/PredType/Basic.lean
@@ -1,0 +1,23 @@
+import LeanMqtt.Core.Codec
+
+namespace Mqtt
+open Mqtt
+
+/--
+  `PredType` is a generic primitive for fields that are only correct when a
+  given predicate is true.
+-/
+abbrev PredType {α : Type} (p : α → Prop) : Type :=
+  { val : α // p val }
+
+def PredType.serialize {α : Type} [c : Codec α] {p : α → Prop} (v : PredType p) : List UInt8 :=
+  @Codec.serialize α c v.val
+
+def PredType.parser {α : Type} [c : Codec α] (p : α → Prop) [DecidablePred p] : Parser (PredType p) := do
+  let val ← @Codec.parser α c
+  if h : p val then
+    return ⟨val, h⟩
+  else
+    failure
+
+end Mqtt
