LeanMqtt/Primitives/PredType/Proofs.lean
@@ -1,0 +1,34 @@
+import LeanMqtt.Primitives.PredType.Basic
+import LeanMqtt.Helpers.ParserTactics
+
+namespace Mqtt
+open Mqtt
+
+theorem PredType.roundtrip {α : Type} [c : Codec α] [LawfulCodec α] {p : α → Prop} [DecidablePred p]
+    (v : PredType p) {rest : List UInt8} :
+    (PredType.parser p).run (PredType.serialize v ++ rest) = some (v, rest) := by
+  unfold PredType.parser PredType.serialize
+  cases v with
+  | mk val property =>
+    have h_round := @LawfulCodec.roundtrip α c _ val rest
+    dsimp [bind, StateT.bind, Option.bind, StateT.run] at *
+    rw [h_round]
+    dsimp
+    rw [dif_pos property]
+    rfl
+
+theorem PredType.reconstruct {α : Type} [c : Codec α] [LawfulCodec α] (p : α → Prop) [DecidablePred p]
+    {v : PredType p} {input rest : List UInt8} :
+    (PredType.parser p).run input = some (v, rest) → input = PredType.serialize v ++ rest := by
+  unfold PredType.parser PredType.serialize
+  intro h
+  step_parser h → val rest' h_val
+  split at h
+  · finish_parser h → h_eq
+    subst h_eq
+    apply @LawfulCodec.reconstruct α c _ val input
+    exact h_val
+  · dsimp [failure, Alternative.failure, StateT.failure, Option.bind] at h
+    contradiction
+
+end Mqtt
