LeanMqtt/Primitives/Proofs.lean
@@ -1,3 +1,7 @@
 import LeanMqtt.Primitives.UInt.Proofs
 import LeanMqtt.Primitives.VarInt.Proofs
 import LeanMqtt.Primitives.Str.Proofs
+import LeanMqtt.Primitives.SizedList.Proofs
+import LeanMqtt.Primitives.OptType.Proofs
+import LeanMqtt.Primitives.ConstVal.Proofs
+import LeanMqtt.Primitives.PredType.Proofs
